Proof skeleton for action refinement.

Subprocess.thy
@@ -4,9 +4,131 @@ imports Main
 
 begin
 
+text "Related to assume-guarantee reasoning, e.g. https://arxiv.org/pdf/2103.13743.pdf"
+text "Goes back to Lamport & Abadi: https://lamport.azurewebsites.net/pubs/abadi-conjoining.pdf"
+
+section "Step function only"
+
+text "Each action operates on its own state, which is defined as a 'v view type that's
+      definable by a lens on the state type. This is different than the seL4 process model,
+      since that effectively only has a single lens whereas multiple lenses are required for
+      each action here."
+
 record ('s, 'v) lens  = 
   Get :: "'s \<Rightarrow> 'v"
   Put :: "'v \<Rightarrow> 's \<Rightarrow> 's"
+
+type_synonym ('e, 's) process = "'e \<Rightarrow> 's \<Rightarrow> 's"
+
+definition exec :: "('e, 's) process \<Rightarrow> 'e list \<Rightarrow> 's \<Rightarrow> 's" where
+"exec step es i = foldl (\<lambda>s e. step e s) i es"
+
+record ('s, 'a) subaction =
+  salens :: "('s, 'a) lens"
+  sastep :: "'a \<Rightarrow> 'a"
+
+type_synonym ('e, 's, 'a) action_mapping = "'e \<Rightarrow> ('s, 'a) subaction"
+
+definition compose_subactions :: "('e, 's, 'a) action_mapping \<Rightarrow> ('e, 's) process"  where
+"compose_subactions spmap = (\<lambda>e s.(
+  let subproc = spmap e in
+  let lns = (salens subproc) in
+  let stp = (sastep subproc) in
+  let v = (Get lns) s in
+  let res = stp v in
+  
+  (Put lns) res s
+))"
+
+(* lemma - a process built with compose_subactions is equivalent to a process defined without it? *)
+
+text "'Action Refinement' is where each isolated implementation action refines its corresponding
+    action in the model. The state type of the step function vfn is local to the action and does
+    not refer to the global state in any way."
+
+definition "single_action_refines proc_i proc_m = (\<forall>ss ss'. proc_i ss = ss' \<longrightarrow> proc_m ss = ss')"
+
+definition "action_refines am_i am_m e =
+  (let proc_i = sastep (am_i e) in 
+  let proc_m = sastep (am_m e) in
+
+  single_action_refines proc_i proc_m)"
+
+definition "refines impl_proc model_proc es = (\<forall>s. exec impl_proc es = s \<longrightarrow> exec model_proc es = s)"
+
+lemma local_refinement:
+  assumes "action_refines am_i am_m e"
+  shows "single_action_refines (sastep (am_i e)) (sastep (am_m e))"
+proof -
+  have "action_refines am_i am_m e" by fact
+  then have "single_action_refines (sastep (am_i e)) (sastep (am_m e))" 
+    unfolding action_refines_def single_action_refines_def
+    by auto
+  then show ?thesis by simp
+qed
+
+lemma composed_subactions_refinement:
+  assumes "\<And> e. e \<in> set es \<Longrightarrow> action_refines am_i am_m e"
+  shows "refines (compose_subactions am_i) (compose_subactions am_m) es"
+proof (induction es)
+  case Nil
+  then show ?case unfolding exec_def refines_def by simp
+next
+  case (Cons e es)
+  from Cons.prems have "action_refines am_i am_m e"  by simp
+  from local_refinement[OF this, of e] have "single_action_refines (sastep (am_i e)) (sastep (am_m e))" by auto
+  with Cons.IH Cons.prems show ?case
+    unfolding refines_def exec_def compose_subactions_def single_action_refines_def
+    by (auto simp add: Let_def)
+qed
+
+theorem main_theorem:
+  assumes "model_proc = compose_subactions am_m"
+    and "impl_proc = compose_subactions am_i"
+    and "\<And>e. e \<in> set es \<Longrightarrow> action_refines am_i am_m e"
+  shows "refines impl_proc model_proc es"
+  using assms composed_subactions_refinement
+  by auto
+
+text "Action refinement implies refinement of the processes with global state, provided that 
+    each process at the global level's step function is defined via the 'compose_subprocs' 
+    function"
+
+text "Need to relate action_refines to global execution"
+
+(* If a model and implementation can be built by composing sub-actions together,
+   and the individal actions refine each other at the local level,
+   then the global implementation refines the global model. *)
+theorem 
+  assumes
+    "model_proc = compose_subactions am_m" and
+    "impl_proc =  compose_subactions am_i" and
+    "action_refines am_i am_m"
+  shows "refines impl_proc model_proc es"
+proof(induction es arbitrary: s am_i am_m)
+  case Nil
+  then show ?case unfolding exec_def refines_def by simp
+next
+  case (Cons a es)
+  then show ?case
+    sorry
+  qed
+
+definition "simulates impl_proc model_proc= (\<forall>e s s'.
+  impl_proc e s = s' \<longrightarrow> model_proc e s = s')"
+
+theorem
+  assumes "simulates I M"
+  shows "refines I M es"
+  oops
+
+
+(* 
+
+GlobalState |> ActionLens.Get |> Action |> ActionLens.Put
+
+*)
+
 
 record ('s, 'e) dt =
   state :: 's
@@ -45,21 +167,12 @@ definition compose_subprocs :: "('e, 's, 'v) subproc_mapping \<Rightarrow> ('e, 
   (Put lns) res s
 ))"
 
-text "'Action Refinement' is where each isolated implementation action refines its corresponding
-    action in the model. The state type of the step function vfn is local to the action and does
-    not refer to the global state in any way."
-
-definition "single_action_refines stp_i stp_m = (\<forall>ss ss'. stp_i ss = ss' \<longrightarrow> stp_m ss = ss')"
-
-definition "action_refines spmi spmm = (\<forall>e.
-  let stp_i = spstep (spmi e) in 
-  let stp_m = spstep (spmm e) in
-
-  single_action_refines stp_i stp_m)"
-
-text "Action refinement implies refinement of the processes with global state, provided that 
-    each process at the global level's step function is defined via the 'compose_subprocs' 
-    function"
+(* Some equivalence between a process and its decomposition into a set of subprocesses"
+theorem
+  assumes "proc = \<lparr> state=s, step=step \<rparr>"
+    and   "subproc = 
+  shows proc_subproc_equiv: "x = y"
+*)
 
 definition "refines_dt C M = (\<forall>s s' es. exec_dt C s es = s' \<longrightarrow> exec_dt M s es = s')"
 
@@ -78,6 +191,7 @@ next
     unfolding compose_subprocs_def action_refines_def single_action_refines_def refines_dt_def 
       exec_dt_def Let_def
     sorry
+   
 qed
 
 section "Subprocs for banking"
